WIP obseq

theories/Typing.v
@@ -179,24 +179,24 @@ Inductive typing : ctx -> level -> term → term → Prop :=
       Γ ⊢< Ax l > t : Lift l A ->
       Γ ⊢< l > lower l A t : A
 
-| type_obseq :
+(* | type_obseq :
     ∀ Γ n A a b,
     Γ ⊢< Ax (ty n) > A : Sort (ty n) ->
     Γ ⊢< ty n > a : A ->
     Γ ⊢< ty n > b : A ->
-    Γ ⊢< Ax prop > obseq (ty n) A a b : Sort prop
+    Γ ⊢< Ax prop > obseq (ty n) A a b : Sort prop *)
 
-| type_obsrefl :
+(* | type_obsrefl :
     ∀ Γ n A a,
       Γ ⊢< Ax (ty n) > A : Sort (ty n) ->
       Γ ⊢< ty n > a : A ->
-      Γ ⊢< prop > obsrefl (ty n) A a : obseq (ty n) A a a
+      Γ ⊢< prop > obsrefl (ty n) A a : obseq (ty n) A a a *)
 
 | type_cast :
     ∀ Γ i A B e a,
     Γ ⊢< Ax i > A : Sort i ->
     Γ ⊢< Ax i > B : Sort i ->
-    Γ ⊢< prop > e : obseq (Ax i) (Sort i) A B ->
+    Γ ⊢< prop > e : Eq (Ax i) (Sort i) A B ->
     Γ ⊢< i > a : A ->
     Γ ⊢< i > cast i A B e a : B
 
@@ -206,8 +206,8 @@ Inductive typing : ctx -> level -> term → term → Prop :=
     Γ ,, (i, A1) ⊢< Ax (ty n) > B1 : Sort (ty n) ->
     Γ ⊢< Ax i > A2 : Sort i ->
     Γ ,, (i, A2) ⊢< Ax (ty n) > B2 : Sort (ty n) ->
-    Γ ⊢< prop > e : obseq (Ax (Ru i (ty n))) (Sort (Ru i (ty n))) (Pi i (ty n) A1 B1) (Pi i (ty n) A2 B2) ->
-    Γ ⊢< prop > injpi1 i (ty n) A1 A2 B1 B2 e : obseq (Ax i) (Sort i) A2 A1
+    Γ ⊢< prop > e : Eq (Ax (Ru i (ty n))) (Sort (Ru i (ty n))) (Pi i (ty n) A1 B1) (Pi i (ty n) A2 B2) ->
+    Γ ⊢< prop > injpi1 i (ty n) A1 A2 B1 B2 e : Eq (Ax i) (Sort i) A2 A1
 
 | type_injpi2 :
   ∀ Γ i n A1 A2 B1 B2 e a2,
@@ -215,10 +215,10 @@ Inductive typing : ctx -> level -> term → term → Prop :=
     Γ ,, (i, A1) ⊢< Ax (ty n) > B1 : Sort (ty n) ->
     Γ ⊢< Ax i > A2 : Sort i ->
     Γ ,, (i, A2) ⊢< Ax (ty n) > B2 : Sort (ty n) ->
-    Γ ⊢< prop > e : obseq (Ax (Ru i (ty n))) (Sort (Ru i (ty n))) (Pi i (ty n) A1 B1) (Pi i (ty n) A2 B2) ->
+    Γ ⊢< prop > e : Eq (Ax (Ru i (ty n))) (Sort (Ru i (ty n))) (Pi i (ty n) A1 B1) (Pi i (ty n) A2 B2) ->
     Γ ⊢< i > a2 : A2 ->
     let a1 := cast i A2 A1 (injpi1 i (ty n) A1 A2 B1 B2 e) a2 in
-    Γ ⊢< prop > injpi2 i (ty n) A1 A2 B1 B2 e a2 : obseq (Ax (ty n)) (Sort (ty n)) (B1<[a1..]) (B2 <[a2..])
+    Γ ⊢< prop > injpi2 i (ty n) A1 A2 B1 B2 e a2 : Eq (Ax (ty n)) (Sort (ty n)) (B1<[a1..]) (B2 <[a2..])
 
 | type_conv :
     ∀ Γ l A B t,
@@ -355,6 +355,39 @@ with conversion : ctx -> level -> term -> term -> term -> Prop :=
       Γ ⊢< Ax l > a ≡ a' : Lift l A ->
       Γ ⊢< l > lower l A a ≡ lower l A' a' : A
 
+
+| conv_cast :
+  ∀ Γ i A A' B B' e e' a a',
+    Γ ⊢< Ax i > A ≡ A' : Sort i ->
+    Γ ⊢< Ax i > B ≡ B' : Sort i ->
+    Γ ⊢< prop > e ≡ e' : Eq (Ax i) (Sort i) A B ->
+    Γ ⊢< i > a ≡ a' : A ->
+    Γ ⊢< i > cast i A B e a ≡ cast i A' B' e' a' : B
+
+| conv_injpi1 :
+  ∀ Γ i n A1 A1' A2 A2' B1 B1' B2 B2' e e',
+    Γ ⊢< Ax i > A1 : Sort i ->
+    Γ ⊢< Ax i > A1 ≡ A1' : Sort i ->
+    Γ ,, (i, A1) ⊢< Ax (ty n) > B1 ≡ B1' : Sort (ty n) ->
+    Γ ⊢< Ax i > A2 : Sort i ->
+    Γ ⊢< Ax i > A2 ≡ A2' : Sort i ->
+    Γ ,, (i, A2) ⊢< Ax (ty n) > B2 ≡ B2' : Sort (ty n) ->
+    Γ ⊢< prop > e ≡ e' : Eq (Ax (Ru i (ty n))) (Sort (Ru i (ty n))) (Pi i (ty n) A1 B1) (Pi i (ty n) A2 B2) ->
+    Γ ⊢< prop > injpi1 i (ty n) A1 A2 B1 B2 e ≡ injpi1 i (ty n) A1' A2' B1' B2' e' : Eq (Ax i) (Sort i) A2 A1
+
+| conv_injpi2 :
+  ∀ Γ i n A1 A1' A2 A2' B1 B1' B2 B2' e e' a2 a2',
+    Γ ⊢< Ax i > A1 : Sort i ->
+    Γ ⊢< Ax i > A1 ≡ A1' : Sort i ->
+    Γ ,, (i, A1) ⊢< Ax (ty n) > B1 ≡ B1' : Sort (ty n) ->
+    Γ ⊢< Ax i > A2 : Sort i ->
+    Γ ⊢< Ax i > A2 ≡ A2' : Sort i ->
+    Γ ,, (i, A2) ⊢< Ax (ty n) > B2 ≡ B2' : Sort (ty n) ->
+    Γ ⊢< prop > e ≡ e' : Eq (Ax (Ru i (ty n))) (Sort (Ru i (ty n))) (Pi i (ty n) A1 B1) (Pi i (ty n) A2 B2) ->
+    Γ ⊢< i > a2 ≡ a2' : A2 ->
+    let a1 := cast i A2 A1 (injpi1 i (ty n) A1 A2 B1 B2 e) a2 in
+    Γ ⊢< prop > injpi2 i (ty n) A1 A2 B1 B2 e a2 ≡ injpi2 i (ty n) A1' A2' B1' B2' e' a2' : Eq (Ax (ty n)) (Sort (ty n)) (B1<[a1..]) (B2 <[a2..])      
+
 | conv_conv :
     ∀ Γ l A B t t',
       Γ ⊢< l > t ≡ t' : A ->
@@ -434,59 +467,31 @@ with conversion : ctx -> level -> term -> term -> term -> Prop :=
       Γ ⊢< Ax (ty n) > a : Lift (ty n) A ->
       Γ ⊢< Ax (ty n) > lift (ty n) A (lower (ty n) A a) ≡ a : Lift (ty n) A
 
-| conv_obseq :
+(* | conv_obseq :
   ∀ Γ n A A' a a' b b',
     Γ ⊢< Ax (ty n) > A ≡ A' : Sort (ty n) ->
     Γ ⊢< ty n > a ≡ a' : A ->
     Γ ⊢< ty n > b ≡ b' : A ->
-    Γ ⊢< Ax prop > obseq (ty n) A a b ≡ obseq (ty n) A' a' b' : Sort prop
+    Γ ⊢< Ax prop > obseq (ty n) A a b ≡ obseq (ty n) A' a' b' : Sort prop *)
 
-| conv_obsrefl :
+(* | conv_obsrefl :
   ∀ n Γ A A' a a',
     Γ ⊢< Ax (ty n) > A ≡ A' : Sort (ty n) ->
     Γ ⊢< ty n > a ≡ a' : A ->
-    Γ ⊢< prop > obsrefl (ty n) A a ≡ obsrefl (ty n) A' a' : obseq (ty n) A a a
+    Γ ⊢< prop > obsrefl (ty n) A a ≡ obsrefl (ty n) A' a' : obseq (ty n) A a a *)
 
-| conv_cast :
-  ∀ Γ i A A' B B' e e' a a',
-    Γ ⊢< Ax i > A ≡ A' : Sort i ->
-    Γ ⊢< Ax i > B ≡ B' : Sort i ->
-    Γ ⊢< prop > e : obseq (Ax i) (Sort i) A B ->
-    Γ ⊢< prop > e' : obseq (Ax i) (Sort i) A' B' ->
-    Γ ⊢< prop > e ≡ e' : obseq (Ax i) (Sort i) A B ->
-    Γ ⊢< i > a ≡ a' : A ->
-    Γ ⊢< i > cast i A B e a ≡ cast i A' B' e' a' : B
 
-| conv_injpi1 :
-  ∀ Γ i n A1 A1' A2 A2' B1 B1' B2 B2' e e',
-    Γ ⊢< Ax i > A1 : Sort i ->
-    Γ ⊢< Ax i > A1 ≡ A1' : Sort i ->
-    Γ ,, (i, A1) ⊢< Ax (ty n) > B1 ≡ B1' : Sort (ty n) ->
-    Γ ⊢< Ax i > A2 : Sort i ->
-    Γ ⊢< Ax i > A2 ≡ A2' : Sort i ->
-    Γ ,, (i, A2) ⊢< Ax (ty n) > B2 ≡ B2' : Sort (ty n) ->
-    Γ ⊢< prop > e ≡ e' : obseq (Ax (Ru i (ty n))) (Sort (Ru i (ty n))) (Pi i (ty n) A1 B1) (Pi i (ty n) A2 B2) ->
-    Γ ⊢< prop > injpi1 i (ty n) A1 A2 B1 B2 e ≡ injpi1 i (ty n) A1' A2' B1' B2' e' : obseq (Ax i) (Sort i) A2 A1
+| conv_cast_univ :
+    ∀ Γ i e a,
+      Γ ⊢< prop > e : Eq (Ax (Ax i)) (Sort (Ax i)) (Sort i) (Sort i) ->
+      Γ ⊢< Ax i > a : Sort i ->
+      Γ ⊢< Ax i > cast (Ax i) (Sort i) (Sort i) e a ≡ a : Sort i
 
-| conv_injpi2 :
-  ∀ Γ i n A1 A1' A2 A2' B1 B1' B2 B2' e e' a2 a2',
-    Γ ⊢< Ax i > A1 : Sort i ->
-    Γ ⊢< Ax i > A1 ≡ A1' : Sort i ->
-    Γ ,, (i, A1) ⊢< Ax (ty n) > B1 ≡ B1' : Sort (ty n) ->
-    Γ ⊢< Ax i > A2 : Sort i ->
-    Γ ⊢< Ax i > A2 ≡ A2' : Sort i ->
-    Γ ,, (i, A2) ⊢< Ax (ty n) > B2 ≡ B2' : Sort (ty n) ->
-    Γ ⊢< prop > e ≡ e' : obseq (Ax (Ru i (ty n))) (Sort (Ru i (ty n))) (Pi i (ty n) A1 B1) (Pi i (ty n) A2 B2) ->
-    Γ ⊢< i > a2 ≡ a2' : A2 ->
-    let a1 := cast i A2 A1 (injpi1 i (ty n) A1 A2 B1 B2 e) a2 in
-    Γ ⊢< prop > injpi2 i (ty n) A1 A2 B1 B2 e a2 ≡ injpi2 i (ty n) A1' A2' B1' B2' e' a2' : obseq (Ax (ty n)) (Sort (ty n)) (B1<[a1..]) (B2 <[a2..])
-
-| conv_cast_refl :
-    ∀ Γ i A e a,
-      Γ ⊢< prop > e : obseq (Ax i) (Sort i) A A ->
-      Γ ⊢< Ax i > A : Sort i ->
-      Γ ⊢< i > a : A ->
-      Γ ⊢< i > cast i A A e a ≡ a : A
+| conv_cast_nat :
+    ∀ Γ e a,
+      Γ ⊢< prop > e : Eq (Ax (ty 0)) (Sort (ty 0)) Nat Nat ->
+      Γ ⊢< ty 0 > a : Nat ->
+      Γ ⊢< ty 0 > cast (ty 0) Nat Nat e a ≡ a : Nat
 
 | conv_cast_pi :
   ∀ Γ i n A1 A2 B1 B2 e f,
@@ -494,7 +499,7 @@ with conversion : ctx -> level -> term -> term -> term -> Prop :=
     Γ ,, (i, A1) ⊢< Ax (ty n) > B1 : Sort (ty n) ->
     Γ ⊢< Ax i > A2 : Sort i ->
     Γ ,, (i, A2) ⊢< Ax (ty n) > B2 : Sort (ty n) ->
-    Γ ⊢< prop > e : obseq (Ax (Ru i (ty n))) (Sort (Ru i (ty n))) (Pi i (ty n) A1 B1) (Pi i (ty n) A2 B2) ->
+    Γ ⊢< prop > e : Eq (Ax (Ru i (ty n))) (Sort (Ru i (ty n))) (Pi i (ty n) A1 B1) (Pi i (ty n) A2 B2) ->
     Γ ⊢< Ru i (ty n) > f : Pi i (ty n) A1 B1 ->
     let A1' := S ⋅ A1 in
     let A2' := S ⋅ A2 in
